printInt system call

platform/Safety.v
@@ -2,6 +2,69 @@ Require Import Bedrock PreAutoSep Sys.
 Import XCAP.
 
 
+Definition goodSize' (n : nat) := (N.of_nat n < 1 + Npow2 32)%N.
+
+Lemma wordToNat_ninj : forall sz (u v : word sz),
+  u <> v
+  -> wordToNat u <> wordToNat v.
+  intros; intro; apply H.
+  assert (natToWord sz (wordToNat u) = natToWord sz (wordToNat v)) by congruence.
+  repeat rewrite natToWord_wordToNat in H1.
+  assumption.
+Qed.
+
+Lemma get_memoryIn' : forall m w init,
+  (wordToNat w < init)%nat
+  -> goodSize' init
+  -> smem_get' (allWordsUpto 32 init) w (memoryIn' m _) = m w.
+  induction init; simpl; intuition.
+  destruct (H.addr_dec $(init) w).
+  unfold H.mem_get, ReadByte.
+  congruence.
+  apply IHinit.
+  apply wordToNat_ninj in n.
+  rewrite wordToNat_natToWord_idempotent in n.
+  omega.
+  generalize H0; clear.
+  unfold goodSize'.
+  generalize (Npow2 32); intros.
+  apply Nlt_out in H0.
+  rewrite N2Nat.inj_add in H0.
+  autorewrite with N in *.
+  pre_nomega.
+  simpl in *.
+  omega.
+  generalize H0; clear.
+  unfold goodSize'.
+  generalize (Npow2 32).
+  intros.
+  nomega.
+Qed.
+
+Lemma pow2_N : forall n,
+  N.of_nat (pow2 n) = Npow2 n.
+  intros.
+  assert (N.to_nat (N.of_nat (pow2 n)) = N.to_nat (Npow2 n)).
+  autorewrite with N.
+  symmetry; apply Npow2_nat.
+  assert (N.of_nat (N.to_nat (N.of_nat (pow2 n))) = N.of_nat (N.to_nat (Npow2 n))) by congruence.
+  autorewrite with N in *.
+  assumption.
+Qed.
+
+Lemma get_memoryIn : forall m w,
+  smem_get w (memoryIn m) = m w.
+  intros.
+  unfold smem_get, memoryIn, HT.memoryIn, H.all_addr.
+  rewrite allWords_eq.
+  apply get_memoryIn'.
+  apply wordToNat_bound.
+  hnf.
+  rewrite pow2_N.
+  reflexivity.
+Qed.
+
+
 Section OpSem.
   Variable m : module.
   Variable stn : settings.
@@ -12,8 +75,10 @@ Section OpSem.
     -> l1 = l2.
 
   Definition labelSys (l : LabelMap.key) (pre : assert) :=
-    l = ("sys", Global "abort")
-    /\ pre = Precondition abortS None.
+    (l = ("sys", Global "abort")
+      /\ pre = Precondition abortS None)
+    \/ (l = ("sys", Global "printInt")
+      /\ pre = Precondition printIntS None).
 
   Hypothesis impSys :
     LabelMap.fold (fun l pre P => labelSys l pre /\ P) (Imports m) True.
@@ -52,54 +117,221 @@ Section OpSem.
 
   Hypothesis ok : moduleOk m.
 
-  Hint Constructors reachable sys_step.
+  Hint Constructors reachable sys_step sys_reachable.
 
-  Lemma reachable_sys : forall st st',
-    sys_reachable stn prog st st'
-    -> reachable stn prog st st'
-    \/ (reachable stn prog st st'
-      /\ Labels stn ("sys", Global "abort") = Some (fst st')).
-    induction 1; intuition.
+  Definition goodState (st : state') :=
+    exists l pre, Labels stn l = Some (fst st)
+      /\ interp (specs m stn) (pre (stn, snd st))
+      /\ (LabelMap.MapsTo l pre (Imports m)
+        \/ exists bl, LabelMap.MapsTo l (pre, bl) (Blocks m)).
 
-    destruct H; eauto.
+  Lemma locals_mapped' : forall specs stn st vs ns sp P,
+    interp specs (![array (toArray ns vs) sp * P] (stn, st))
+    -> mapped sp (length ns * 4) (Mem st).
+    induction ns; simpl; intuition; hnf; intuition.
+    unfold array in H.
+    assert (interp specs (![ptsto32m' nil sp 0 (vs a :: toArray ns vs) * P] (stn0, st))).
+    eapply ILTacCommon.interp_interp_himp; eauto.
+    eapply himp_star_frame; [ apply Arrays.ptsto32m'_in | reflexivity ].
+    clear H.
+    simpl in *.
+    assert (n < 4 \/ (n >= 4 /\ n - 4 < length ns * 4))%nat by omega.
+    intuition.
+    rewrite sepFormula_eq in H2; propxFo.
+    unfold smem_get_word, H.footprint_w in H6.
+    repeat match type of H6 with
+             | match ?E with None => _ | _ => _ end = _ => case_eq E; intros;
+               try match goal with
+                     | [ H : _ = _ |- _ ] => rewrite H in H6
+                   end; try discriminate
+           end.
+    inversion H3; clear H3; subst.
 
-    destruct H; eauto.
+    Lemma unsplit_smem_get' : forall a v ls m m',
+      smem_get' ls a m = Some v
+      -> smem_get' ls a (join' ls m m') = Some v.
+      induction ls; simpl; intuition.
+      destruct (H.addr_dec a0 a); subst.
+      rewrite H; auto.
+      eauto.
+    Qed.
+
+    Lemma unsplit_smem_get : forall a m v m0 m1,
+      smem_get a m = Some v
+      -> split m0 m m1
+        -> smem_get a m0 = Some v.
+      unfold split; intuition subst; apply unsplit_smem_get'; auto.
+    Qed.
+
+    do 2 (eapply unsplit_smem_get in H11; eauto).
+    rewrite get_memoryIn in H11.
+    replace (sp ^+ $0 ^+ $3) with (sp ^+ $3) in * by words.
+    congruence.
+
+    inversion H13; clear H13; subst.
+    do 2 (eapply unsplit_smem_get in H10; eauto).
+    rewrite get_memoryIn in H10.
+    replace (sp ^+ $0 ^+ $2) with (sp ^+ $2) in * by words.
+    congruence.
+
+    inversion H12; clear H12; subst.
+    do 2 (eapply unsplit_smem_get in H9; eauto).
+    rewrite get_memoryIn in H9.
+    replace (sp ^+ $0 ^+ $1) with (sp ^+ $1) in * by words.
+    congruence.
+
+    inversion H13; clear H13; subst.
+    do 2 (eapply unsplit_smem_get in H; eauto).
+    rewrite get_memoryIn in H.
+    congruence.
+
+    inversion H12.
+
+    assert (interp specs (![array (toArray ns vs) (sp ^+ $4) * ((sp ^+ $ (0)) =*> vs a * P)] (stn0, st))).
+    eapply ILTacCommon.interp_interp_himp; eauto.
+    clear.
+
+    Lemma comeOnOut : forall P Q R,
+      P * Q * R ===> Q * (P * R).
+      clear; sepLemma.
+    Qed.
+
+    etransitivity; [ apply comeOnOut | ].
+    apply Himp_star_frame; [ | apply Himp_refl ].
+    eapply Himp_trans; [ | apply ptsto32m'_out ].
+    apply ptsto32m'_shift_base'; auto.
+
+    clear H2.
+    apply IHns in H3.
+    hnf in H3.
+    eapply H3.
+    eauto.
+    replace (sp ^+ $4 ^+ $(n - 4)) with (sp ^+ $(n)); auto.
+    rewrite natToW_minus by auto.
+    unfold natToW.
+    W_eq.
   Qed.
 
-  Lemma safe_sys : forall st,
-    safe stn prog st
-    -> sys_safe stn prog st.
-    unfold sys_safe; post.
-    apply reachable_sys in H0; post.
+  Lemma locals_mapped : forall specs ns vs res sp stn st P,
+    interp specs (![locals ns vs res sp * P] (stn, st))
+    -> mapped sp (length ns * 4) (Mem st).
+    unfold locals; intros.
+    assert (interp specs
+      (![array (toArray ns vs) sp * ([|NoDup ns|] *
+        (sp ^+ $ (Datatypes.length ns * 4)) =?> res * P)]
+      (stn0, st))).
+    generalize H; clear; intros; step auto_ext.
+    eapply locals_mapped'; eauto.
+  Qed.
 
-    specialize (H _ H1).
-    case_eq (step stn prog st'); intuition eauto.
+  Lemma specs_hit : forall w pre,
+    specs m stn w = Some pre
+    -> exists l, Labels stn l = Some w
+      /\ (LabelMap.MapsTo l pre (Imports m)
+        \/ exists bl, LabelMap.MapsTo l (pre, bl) (Blocks m)).
+    intros.
+    apply specs_hit in H; post; eauto.
+    apply specs'_hit in H0; post; eauto.
+  Qed.
 
-    specialize (H _ H0).
-    unfold step in H.
-    apply omitImp in H2.
-    rewrite H2 in *.
-    tauto.
+  Lemma progress : forall st, goodState st
+    -> exists st', sys_step stn prog st st'.
+    unfold goodState; post.
+
+    specialize (impSys' _ _ H1); intro Hi; hnf in Hi; intuition subst.
+    eauto 10.
+    post.
+    match goal with
+      | [ H : interp ?specs (![?P * ?Q * ?R] ?X) |- _ ] =>
+        let H' := fresh in
+          assert (H' :interp specs (![P * (Q * R)] X)) by (generalize H; clear; intros; step auto_ext);
+            clear H; rename H' into H
+    end.
+    specialize (locals_mapped _ _ _ _ _ _ _ _ H2); intro Hm; simpl in Hm.
+    apply specs_hit in H3; post; eauto.
+
+    specialize (BlocksOk ok H1); intro Hb; hnf in Hb.
+    apply Hb in H; [ | eapply specsOk; eauto ].
+    clear Hb; post.
+    specialize (agree _ _ _ H1); destruct agree as [ ? [ ] ].
+    rewrite H0 in H; injection H; clear H; intros; subst.
+    apply specs_hit in H3; destruct H3; intuition idtac.
+    descend.
+    apply Normal.
+    unfold step.
+    rewrite H5.
+    eauto.
+
+    destruct H.
+    descend.
+    apply Normal.
+    unfold step.
+    rewrite H5.
+    eauto.
+  Qed.
+
+  Lemma preservation : forall st, goodState st
+    -> forall st', sys_step stn prog st st'
+      -> goodState st'.
+    unfold goodState; destruct 2; post.
+
+    specialize (impSys' _ _ H2); intro Hi; hnf in Hi; intuition subst.
+    apply omitImp in H1.
+    unfold step in H0.
+    rewrite H1 in H0; discriminate.
+    apply omitImp in H1.
+    unfold step in H0.
+    rewrite H1 in H0; discriminate.
+
+    specialize (BlocksOk ok H2); intro Hb; hnf in Hb.
+    apply Hb in H; [ | eapply specsOk; eauto ].
+    clear Hb; post.
+    specialize (agree _ _ _ H2); destruct agree as [ ? [ ] ].
+    rewrite H1 in H; injection H; clear H; intros; subst.
+    unfold step in H0.
+    rewrite H6 in H0.
+    rewrite H0 in H3; injection H3; clear H3; intros; subst.
+    apply specs_hit in H4; destruct H4; intuition idtac.
+    eauto 10.
+    destruct H; eauto 10.
+
+    specialize (impSys' _ _ H3); intro Hi; hnf in Hi; intuition subst.
+    eapply (inj _ _ _ H0) in H2; discriminate. 
+    post.
+    apply specs_hit in H5; destruct H5; intuition idtac.
+    descend.
+    eauto.
+    2: eauto.
+    descend; step auto_ext.
+    descend; eauto.
+    descend.
+    eauto.
+    2: eauto.
+    descend; step auto_ext.
+    descend; eauto.
+
+    apply (inj _ _ _ H0) in H2.
+    subst.
+    specialize (omitImp _ _ H0).
+    apply agree in H3.
+    post.
+    congruence.
+  Qed.
+
+  Lemma safety' : forall st, goodState st
+    -> forall st', sys_reachable stn prog st st'
+      -> goodState st'.
+    induction 2; simpl; eauto using preservation.
   Qed.
 
   Theorem safety : forall st mn g pre, LabelMap.MapsTo (mn, Global g) pre (Exports m)
     -> Labels stn (mn, Global g) = Some (fst st)
     -> interp (specs0 m stn) (pre (stn, snd st))
     -> sys_safe stn prog st.
-    intros; hnf; intros.
-
-    apply (ExportsSound ok) in H; destruct H.
-
-    apply reachable_sys in H2; post.
-    eapply safety'' in H3; eauto.
-    post.
-
-    specialize (impSys' _ _ H4); intro.
-    hnf in H2; intuition subst.
-    apply agreeImp in H4; post; subst.
-    eauto.
-    case_eq (step stn prog st'); intros; eauto; congruence.
-    
-    eauto.
+    unfold sys_safe; intros.
+    eapply safety' in H2.
+    auto using progress.
+    hnf; descend; eauto.
+    apply (ExportsSound ok) in H; eauto.
   Qed.
 End OpSem.
